src/theory/tools/symbexec/birs_rulesScript.sml
@@ -55,6 +55,48 @@ REWRITE_TAC [symb_rulesTheory.symb_pcondwiden_def, birs_pcondwiden_def] >>
   SIMP_TAC (std_ss++symb_TYPES_ss) [bir_symb_rec_sbir_def, symb_interpr_symbpcond_def, bir_bool_expTheory.bir_val_TF_dist]
 QED
 
+(* ******************************************************* *)
+(*      sound execution structure for SBIR                 *)
+(* ******************************************************* *)
+Definition birs_symb_exec_def:
+  birs_symb_exec p (bs, L, bP) =
+      (symb_hl_step_in_L_sound (bir_symb_rec_sbir p) (birs_symb_to_symbst bs, L, IMAGE birs_symb_to_symbst bP))
+End
+
+
+(* ******************************************************* *)
+(*      FREE SYMBS                                         *)
+(* ******************************************************* *)
+Definition birs_symb_symbols_set_def:
+  birs_symb_symbols_set Pi =
+      BIGUNION (IMAGE birs_symb_symbols Pi)
+End
+
+Theorem birs_symb_symbols_set_EQ_thm2:
+  !prog Pi. symb_symbols_set (bir_symb_rec_sbir prog) (IMAGE birs_symb_to_symbst Pi) = birs_symb_symbols_set Pi
+Proof
+  REWRITE_TAC [birs_auxTheory.symb_symbols_set_ALT_thm, birs_symb_symbols_set_def] >>
+  REWRITE_TAC [pred_setTheory.IMAGE_IMAGE, combinTheory.o_DEF, birs_symb_symbols_EQ_thm] >>
+  METIS_TAC []
+  (* birs_symb_symbols_set_EQ_thm *)
+QED
+
+Definition birs_freesymbs_def:
+  birs_freesymbs bs sbs =
+      ((BIGUNION (IMAGE birs_symb_symbols sbs)) DIFF (birs_symb_symbols bs))
+End
+
+Theorem birs_freesymbs_EQ_thm:
+  !prog L bs sbs.
+  birs_freesymbs bs sbs = symb_freesymbs (bir_symb_rec_sbir prog) (birs_symb_to_symbst bs, L, IMAGE birs_symb_to_symbst sbs)
+Proof
+  REWRITE_TAC [birs_freesymbs_def, symb_freesymbs_def] >>
+  REWRITE_TAC [birs_auxTheory.symb_symbols_set_ALT_thm] >>
+  REWRITE_TAC [pred_setTheory.IMAGE_IMAGE, combinTheory.o_DEF, birs_symb_symbols_EQ_thm] >>
+  METIS_TAC []
+QED
+
+
 
 (* ******************************************************* *)
 (*      ASSERT statement justification                     *)
@@ -106,9 +148,9 @@ QED
 
 
 Theorem assert_spec_thm:
-  !bprog sys L lbl1 env1 status pre cond lbl2 env2.
-  (symb_hl_step_in_L_sound (bir_symb_rec_sbir bprog)
-    (sys, L, IMAGE birs_symb_to_symbst {
+  !bprog bs L lbl1 env1 status pre cond lbl2 env2.
+  (birs_symb_exec bprog
+    (bs, L, {
       <|bsst_pc := lbl1;
         bsst_environ := env1;
         bsst_status := status;
@@ -122,14 +164,15 @@ Theorem assert_spec_thm:
    status <> BST_AssertionViolated) ==>
   (birs_pcondinf (BExp_BinExp BIExp_And pre
                  (BExp_UnaryExp BIExp_Not cond))) ==>
-  (symb_hl_step_in_L_sound (bir_symb_rec_sbir bprog)
-    (sys, L, IMAGE birs_symb_to_symbst {
+  (birs_symb_exec bprog
+    (bs, L, {
       <|bsst_pc := lbl1;
         bsst_environ := env1;
         bsst_status := status;
         bsst_pcond := pre|>}))
 Proof
-REPEAT STRIP_TAC >> (
+    REWRITE_TAC [birs_symb_exec_def] >>
+    REPEAT STRIP_TAC >> (
     IMP_RES_TAC symb_rulesTheory.symb_rule_INF_thm >>
     PAT_X_ASSUM ``!x. A`` (ASSUME_TAC o SPEC ``birs_symb_to_symbst <|bsst_pc := lbl2; bsst_environ := env2;
                   bsst_status := BST_AssertionViolated;
@@ -146,6 +189,7 @@ REPEAT STRIP_TAC >> (
     FULL_SIMP_TAC (std_ss++symb_TYPES_ss) [symb_symbst_pcond_def, DIFF_INSERT, DIFF_EMPTY, DELETE_INSERT, EMPTY_DELETE] >>
     REV_FULL_SIMP_TAC (std_ss) [] >>
 
+    Q.ABBREV_TAC `sys = SymbSymbSt bs.bsst_pc bs.bsst_environ bs.bsst_pcond bs.bsst_status` >>
     Q.ABBREV_TAC `sys2 = SymbSymbSt lbl1 env1 (BExp_BinExp BIExp_And pre cond) status` >>
     Q.ABBREV_TAC `sys2' = SymbSymbSt lbl1 env1 pre status` >>
 
@@ -171,9 +215,9 @@ QED
 
 
 Theorem branch_prune1_spec_thm:
-  !bprog sys L lbl1 env1 status1 pre cond lbl2 env2 status2.
-  (symb_hl_step_in_L_sound (bir_symb_rec_sbir bprog)
-    (sys, L, IMAGE birs_symb_to_symbst {
+  !bprog bs L lbl1 env1 status1 pre cond lbl2 env2 status2.
+  (birs_symb_exec bprog
+    (bs, L, {
       <|bsst_pc := lbl1;
         bsst_environ := env1;
         bsst_status := status1;
@@ -186,14 +230,15 @@ Theorem branch_prune1_spec_thm:
   (lbl1 <> lbl2 \/
    status1 <> status2) ==>
   (birs_pcondinf (BExp_BinExp BIExp_And pre cond)) ==>
-  (symb_hl_step_in_L_sound (bir_symb_rec_sbir bprog)
-    (sys, L, IMAGE birs_symb_to_symbst {
+  (birs_symb_exec bprog
+    (bs, L, {
       <|bsst_pc := lbl2;
         bsst_environ := env2;
         bsst_status := status2;
         bsst_pcond := BExp_BinExp BIExp_And pre
                  (BExp_UnaryExp BIExp_Not cond)|>}))
 Proof
+  REWRITE_TAC [birs_symb_exec_def] >>
   REPEAT STRIP_TAC >> (
     IMP_RES_TAC symb_rulesTheory.symb_rule_INF_thm >>
     PAT_X_ASSUM ``!x. A`` (ASSUME_TAC o SPEC ``birs_symb_to_symbst <|bsst_pc := lbl1;
@@ -215,9 +260,9 @@ QED
 
 
 Theorem branch_prune2_spec_thm:
-  !bprog sys L lbl1 env1 status1 pre cond lbl2 env2 status2.
-  (symb_hl_step_in_L_sound (bir_symb_rec_sbir bprog)
-    (sys, L, IMAGE birs_symb_to_symbst {
+  !bprog bs L lbl1 env1 status1 pre cond lbl2 env2 status2.
+  (birs_symb_exec bprog
+    (bs, L, {
       <|bsst_pc := lbl1;
         bsst_environ := env1;
         bsst_status := status1;
@@ -231,14 +276,15 @@ Theorem branch_prune2_spec_thm:
    status1 <> status2) ==>
   (birs_pcondinf (BExp_BinExp BIExp_And pre
                  (BExp_UnaryExp BIExp_Not cond))) ==>
-  (symb_hl_step_in_L_sound (bir_symb_rec_sbir bprog)
-    (sys, L, IMAGE birs_symb_to_symbst {
+  (birs_symb_exec bprog
+    (bs, L, {
       <|bsst_pc := lbl1;
         bsst_environ := env1;
         bsst_status := status1;
         bsst_pcond := BExp_BinExp BIExp_And pre cond|>}))
 Proof
-  REPEAT STRIP_TAC >> (
+    REWRITE_TAC [birs_symb_exec_def] >>
+    REPEAT STRIP_TAC >> (
     IMP_RES_TAC symb_rulesTheory.symb_rule_INF_thm >>
     PAT_X_ASSUM ``!x. A`` (ASSUME_TAC o SPEC ``birs_symb_to_symbst <|bsst_pc := lbl2;
         bsst_environ := env2;
@@ -285,24 +331,25 @@ REPEAT STRIP_TAC >>
 QED
 
 Theorem birs_rule_SUBST_spec_thm:
-  !prog sys L sys2 sys2' lbl envl status pcond vn symbexp symbexp'.
-           (sys2 =
+  !prog bs L bs2 bs2' lbl envl status pcond vn symbexp symbexp'.
+           (bs2 =
              <|bsst_pc := lbl;
                bsst_environ := birs_gen_env ((vn, symbexp)::envl);
                bsst_status := status;
                bsst_pcond := pcond|>) ==>
-           (sys2' =
+           (bs2' =
              <|bsst_pc := lbl;
                bsst_environ := birs_gen_env ((vn, symbexp')::envl);
                bsst_status := status;
                bsst_pcond := pcond|>) ==>
-           symb_hl_step_in_L_sound (bir_symb_rec_sbir prog) (sys,L,IMAGE birs_symb_to_symbst {sys2}) ==>
+           birs_symb_exec prog (bs, L, {bs2}) ==>
            birs_simplification pcond symbexp symbexp' ==>
-           symb_hl_step_in_L_sound (bir_symb_rec_sbir prog) (sys,L,IMAGE birs_symb_to_symbst {sys2'})
+           birs_symb_exec prog (bs, L, {bs2'})
 Proof
-REPEAT STRIP_TAC >>
+  REWRITE_TAC [birs_symb_exec_def] >>
+  REPEAT STRIP_TAC >>
   ASSUME_TAC (
-    (Q.SPECL [`sys`, `L`, `birs_symb_to_symbst sys2`, `vn`, `symbexp`, `symbexp'`] o
+    (Q.SPECL [`birs_symb_to_symbst bs`, `L`, `birs_symb_to_symbst bs2`, `vn`, `symbexp`, `symbexp'`] o
      SIMP_RULE std_ss [bir_symb_soundTheory.birs_symb_ARB_val_sound_thm] o
      MATCH_MP symb_rule_SUBST_SING_thm o
      Q.SPEC `prog`)
@@ -344,55 +391,18 @@ Theorem birs_rule_STEP_gen2_thm:
   !prog bsys.
   (bir_prog_has_no_halt prog) ==>
 
-  (symb_hl_step_in_L_sound (bir_symb_rec_sbir prog)
-    (birs_symb_to_symbst bsys,
+  (birs_symb_exec prog
+    (bsys,
      {bsys.bsst_pc},
-     IMAGE birs_symb_to_symbst
-       (birs_exec_step prog bsys)))
+     (birs_exec_step prog bsys)))
 Proof
-REPEAT STRIP_TAC >>
+  REWRITE_TAC [birs_symb_exec_def] >>
+  REPEAT STRIP_TAC >>
   IMP_RES_TAC birs_rule_STEP_gen1_thm >>
   POP_ASSUM (ASSUME_TAC o Q.SPEC `birs_symb_to_symbst bsys`) >>
 
   FULL_SIMP_TAC std_ss [bir_symbTheory.birs_symb_to_from_symbst_thm, birs_auxTheory.birs_symb_symbst_pc_thm]
 QED
-
-
-(* ******************************************************* *)
-(*      FREE SYMBS                                         *)
-(* ******************************************************* *)
-Definition birs_symb_symbols_set_def:
-  birs_symb_symbols_set Pi =
-      BIGUNION (IMAGE birs_symb_symbols Pi)
-End
-
-Theorem birs_symb_symbols_set_EQ_thm:
-  !prog Pi. symb_symbols_set (bir_symb_rec_sbir prog) (IMAGE birs_symb_to_symbst Pi) = birs_symb_symbols_set Pi
-Proof
-  REWRITE_TAC [birs_auxTheory.symb_symbols_set_ALT_thm, birs_symb_symbols_set_def] >>
-  REWRITE_TAC [pred_setTheory.IMAGE_IMAGE, combinTheory.o_DEF, birs_symb_symbols_EQ_thm] >>
-  METIS_TAC []
-QED
-
-Definition birs_freesymbs_def:
-  birs_freesymbs bs sbs =
-      ((BIGUNION (IMAGE birs_symb_symbols sbs)) DIFF (birs_symb_symbols bs))
-End
-
-Theorem birs_freesymbs_EQ_thm:
-  !prog L bs sbs.
-  birs_freesymbs bs sbs = symb_freesymbs (bir_symb_rec_sbir prog) (birs_symb_to_symbst bs, L, IMAGE birs_symb_to_symbst sbs)
-Proof
-  REWRITE_TAC [birs_freesymbs_def, symb_freesymbs_def] >>
-  REWRITE_TAC [birs_auxTheory.symb_symbols_set_ALT_thm] >>
-  REWRITE_TAC [pred_setTheory.IMAGE_IMAGE, combinTheory.o_DEF, birs_symb_symbols_EQ_thm] >>
-  METIS_TAC []
-QED
-
-Definition birs_freesymbs_SING_def:
-  birs_freesymbs_SING bs1 bs2 =
-      ((birs_symb_symbols bs2) DIFF (birs_symb_symbols bs1))
-End
 
 
 (* ******************************************************* *)
@@ -414,28 +424,70 @@ val betterTheorem = prove(``
   METIS_TAC[symb_rulesTheory.symb_rule_SEQ_thm]
 );
 
+val IMAGE_DIFF_ASSOC_thm = prove(``
+!f s1 s2.
+  (!x y. f x = f y <=> x = y) ==>
+  ((IMAGE f s1) DIFF (IMAGE f s2) =
+   IMAGE f (s1 DIFF s2))
+``,
+    fs [IMAGE_DEF, DIFF_DEF, EXTENSION] >>
+    REPEAT STRIP_TAC >>
+    EQ_TAC >> (
+      METIS_TAC []
+    )
+);
+
+val IMAGE_UNION_ASSOC_thm = prove(``
+!f s1 s2.
+  (!x y. f x = f y <=> x = y) ==>
+  ((IMAGE f s1) UNION (IMAGE f s2) =
+   IMAGE f (s1 UNION s2))
+``,
+    fs [IMAGE_DEF, UNION_DEF, EXTENSION] >>
+    REPEAT STRIP_TAC >>
+    EQ_TAC >> (
+      METIS_TAC []
+    )
+);
+
+val bestTheorem = prove(“
+ !A B C.
+  IMAGE birs_symb_to_symbst A DIFF {birs_symb_to_symbst B} UNION IMAGE birs_symb_to_symbst C =
+  IMAGE birs_symb_to_symbst (A DIFF {B} UNION C)
+”,
+  REWRITE_TAC [GSYM IMAGE_SING] >>
+  REWRITE_TAC
+    [MATCH_MP IMAGE_DIFF_ASSOC_thm birs_symb_to_symbst_EQ_thm,
+     MATCH_MP IMAGE_UNION_ASSOC_thm birs_symb_to_symbst_EQ_thm]
+);
+
 Theorem birs_rule_SEQ_gen_thm:
   !prog bsys_A L_A bPi_A bsys_B L_B bPi_B.
-  (symb_hl_step_in_L_sound (bir_symb_rec_sbir prog) (birs_symb_to_symbst bsys_A, L_A, IMAGE birs_symb_to_symbst bPi_A)) ==>
-  (symb_hl_step_in_L_sound (bir_symb_rec_sbir prog) (birs_symb_to_symbst bsys_B, L_B, IMAGE birs_symb_to_symbst bPi_B)) ==>
+  (birs_symb_exec prog (bsys_A, L_A, bPi_A)) ==>
+  (birs_symb_exec prog (bsys_B, L_B, bPi_B)) ==>
 
   ((birs_symb_symbols bsys_A) INTER (birs_freesymbs bsys_B bPi_B) = EMPTY) ==>
 
-  (*(symb_hl_step_in_L_sound (bir_symb_rec_sbir prog) (birs_symb_to_symbst bsys_A, L_A UNION L_B, IMAGE birs_symb_to_symbst ((bPi_A DIFF {bsys_B}) UNION bPi_B))) *)
-  (symb_hl_step_in_L_sound (bir_symb_rec_sbir prog) (birs_symb_to_symbst bsys_A, L_A UNION L_B, ((IMAGE birs_symb_to_symbst bPi_A) DIFF {birs_symb_to_symbst bsys_B}) UNION (IMAGE birs_symb_to_symbst bPi_B)))
+  (birs_symb_exec prog (bsys_A, L_A UNION L_B, (bPi_A DIFF {bsys_B}) UNION bPi_B))
 Proof
+  REWRITE_TAC [birs_symb_exec_def] >>
   REPEAT GEN_TAC >>
   REWRITE_TAC [ISPECL [``prog: 'a bir_program_t``, ``L_B:bir_programcounter_t -> bool``, ``bsys_B:birs_state_t``, ``bPi_B:birs_state_t -> bool``] birs_freesymbs_EQ_thm] >>
   REWRITE_TAC [GSYM birs_symb_symbols_EQ_thm] >>
   REPEAT STRIP_TAC >>
   ASSUME_TAC (ISPEC ``prog: 'a bir_program_t`` bir_symb_soundTheory.birs_symb_symbols_f_sound_thm) >>
-  METIS_TAC [betterTheorem]
+  METIS_TAC [betterTheorem, bestTheorem]
 QED
 
 
 (* ******************************************************* *)
 (*      NO FREE SYMBS                                      *)
 (* ******************************************************* *)
+Definition birs_freesymbs_SING_def:
+  birs_freesymbs_SING bs1 bs2 =
+      ((birs_symb_symbols bs2) DIFF (birs_symb_symbols bs1))
+End
+
 Definition birs_freesymbs_EMPTY_def:
   birs_freesymbs_EMPTY bs sbs =
       (birs_freesymbs bs sbs = EMPTY)
@@ -836,41 +888,41 @@ QED
 (*      STEP SEQ rule                                      *)
 (* ******************************************************* *)
 Theorem birs_rule_STEP_SEQ_gen_thm:
-  !prog bsys1 L bsys2.
+  !prog bs1 L bs2.
   (bir_prog_has_no_halt prog) ==>
 
-  (symb_hl_step_in_L_sound (bir_symb_rec_sbir prog)
-    (birs_symb_to_symbst bsys1,
+  (birs_symb_exec prog
+    (bs1,
      L,
-     IMAGE birs_symb_to_symbst {bsys2}
+     {bs2}
   )) ==>
 
-  (symb_hl_step_in_L_sound (bir_symb_rec_sbir prog)
-    (birs_symb_to_symbst bsys1,
-     (bsys2.bsst_pc) INSERT L,
-     IMAGE birs_symb_to_symbst (birs_exec_step prog bsys2)
+  (birs_symb_exec prog
+    (bs1,
+     (bs2.bsst_pc) INSERT L,
+     (birs_exec_step prog bs2)
   ))
 Proof
+  REWRITE_TAC [birs_symb_exec_def] >>
   REPEAT STRIP_TAC >>
 
-  ASSUME_TAC (Q.SPECL [`prog`, `bsys2`] birs_rule_STEP_gen2_thm) >>
-  REV_FULL_SIMP_TAC std_ss [] >>
-
+  ASSUME_TAC (Q.SPECL [`prog`, `bs2`] birs_rule_STEP_gen2_thm) >>
+  REV_FULL_SIMP_TAC std_ss [birs_symb_exec_def] >>
 
   ASSUME_TAC (Q.SPEC `prog` bir_symb_soundTheory.birs_symb_symbols_f_sound_thm) >>
   IMP_RES_TAC (REWRITE_RULE [symb_freesymbs_def] symb_rulesTheory.symb_rule_SEQ_thm) >>
-  POP_ASSUM (ASSUME_TAC o Q.SPECL [`birs_symb_to_symbst bsys2`, `birs_symb_to_symbst bsys1`, `IMAGE birs_symb_to_symbst (birs_exec_step prog bsys2)`]) >>
+  POP_ASSUM (ASSUME_TAC o Q.SPECL [`birs_symb_to_symbst bs2`, `birs_symb_to_symbst bs1`, `IMAGE birs_symb_to_symbst (birs_exec_step prog bs2)`]) >>
   ASSUME_TAC (REWRITE_RULE [birs_freesymbs_EMPTY_def, birs_freesymbs_def] birs_exec_step_NO_FRESH_SYMBS) >>
   FULL_SIMP_TAC std_ss [INTER_EMPTY,
     birs_auxTheory.birs_symb_symbols_set_EQ_thm, bir_symb_sound_coreTheory.birs_symb_symbols_EQ_thm] >>
 
-  `L UNION {bsys2.bsst_pc} = bsys2.bsst_pc INSERT L` by (
+  `L UNION {bs2.bsst_pc} = bs2.bsst_pc INSERT L` by (
     METIS_TAC [INSERT_UNION_EQ, UNION_EMPTY, UNION_COMM]
   ) >>
 
-  `(IMAGE birs_symb_to_symbst {bsys2} DIFF {birs_symb_to_symbst bsys2}) UNION
-               IMAGE birs_symb_to_symbst (birs_exec_step prog bsys2)
-   = IMAGE birs_symb_to_symbst (birs_exec_step prog bsys2)` by (
+  `(IMAGE birs_symb_to_symbst {bs2} DIFF {birs_symb_to_symbst bs2}) UNION
+               IMAGE birs_symb_to_symbst (birs_exec_step prog bs2)
+   = IMAGE birs_symb_to_symbst (birs_exec_step prog bs2)` by (
     SIMP_TAC std_ss [IMAGE_INSERT, IMAGE_EMPTY, DIFF_EQ_EMPTY, UNION_EMPTY]
   ) >>
 
