src/tools/symbexec/birs_composeLib.sml
@@ -44,6 +44,7 @@ fun birs_rule_SEQ_prog_fun bprog_tm =
   *)
 
 (* symbol freedom helper function *)
+(* probably should remove the parameter freesymbols_B_thm_o, because obsolete since we have a special STEP_SEQ rule *)
 fun birs_rule_SEQ_free_symbols_fun freesymbols_tm freesymbols_B_thm_o =
   let
 
@@ -58,32 +59,12 @@ fun birs_rule_SEQ_free_symbols_fun freesymbols_tm freesymbols_B_thm_o =
           NONE => ALL_TAC
         | SOME freesymbols_B_thm => (print_thm freesymbols_B_thm; raise ERR "" ""; REWRITE_TAC [freesymbols_B_thm, pred_setTheory.INTER_EMPTY])) >>
 
-      FULL_SIMP_TAC (std_ss) [bir_symb_sound_coreTheory.birs_symb_symbols_EQ_thm, birs_symb_symbols_set_EQ_thm] >>
+      FULL_SIMP_TAC (std_ss) [birs_rulesTheory.birs_symb_symbols_set_def, birs_rulesTheory.birs_freesymbs_def] >>
 
-      (* TODO *)
+      (* this is to unfold the definitions within the states (env_list_gen) so that the vars_of_symbol function can work *)
       CONV_TAC (computeLib.RESTR_EVAL_CONV [``birs_symb_symbols``, ``$BIGUNION``]) >>
 
-
-
       CONV_TAC (bir_vars_ofLib.birs_symb_symbols_CONV) >>
-(*
-      CONV_TAC (
-  SIMP_CONV (std_ss++birs_state_ss) [birs_symb_symbols_thm] THENC
-
-
-  GEN_match_conv is_birs_exps_of_senv birs_exps_of_senv_CONV THENC
-(*
-  REWRITE_CONV [birs_exps_of_senv_thm] THENC
-*)
-  REWRITE_CONV [bir_typing_expTheory.bir_vars_of_exp_def] THENC
-
-  computeLib.RESTR_EVAL_CONV [``$DIFF``, ``$INTER``, ``$UNION``, ``$INSERT``, ``$BIGUNION``] THENC
-      REWRITE_CONV [pred_setTheory.BIGUNION_INSERT, pred_setTheory.BIGUNION_EMPTY] THENC
-      REWRITE_CONV [pred_setTheory.UNION_ASSOC, pred_setTheory.INSERT_UNION_EQ, pred_setTheory.UNION_EMPTY] THENC
-
-  REFL
-) >>
-*)
 
       REWRITE_TAC [pred_setTheory.BIGUNION_INSERT, pred_setTheory.BIGUNION_EMPTY] >>
       REWRITE_TAC [pred_setTheory.UNION_ASSOC, pred_setTheory.INSERT_UNION_EQ, pred_setTheory.UNION_EMPTY] >>
@@ -92,105 +73,6 @@ fun birs_rule_SEQ_free_symbols_fun freesymbols_tm freesymbols_B_thm_o =
       (fn (al,g) => (print_term g; ([(al,g)], fn ([t]) => t))) >>
 *)
       (fn (al,g) => (print "starting to proof free symbols\n"; ([(al,g)], fn ([t]) => t))) >>
-
-(*
-prove(``{BVar "sy_tmp_countw" (BType_Imm Bit64);
- BVar "sy_tmp_ModeHandler" (BType_Imm Bit1);
- BVar "sy_tmp_SP_process" (BType_Imm Bit32);
- BVar "sy_tmp_SP_main" (BType_Imm Bit32); BVar "sy_tmp_LR" (BType_Imm Bit32);
- BVar "sy_tmp_R12" (BType_Imm Bit32); BVar "sy_tmp_R11" (BType_Imm Bit32);
- BVar "sy_tmp_R10" (BType_Imm Bit32); BVar "sy_tmp_R9" (BType_Imm Bit32);
- BVar "sy_tmp_R8" (BType_Imm Bit32); BVar "sy_tmp_R7" (BType_Imm Bit32);
- BVar "sy_tmp_R6" (BType_Imm Bit32); BVar "sy_tmp_R5" (BType_Imm Bit32);
- BVar "sy_tmp_R4" (BType_Imm Bit32); BVar "sy_tmp_R3" (BType_Imm Bit32);
- BVar "sy_tmp_R2" (BType_Imm Bit32); BVar "sy_tmp_R1" (BType_Imm Bit32);
- BVar "sy_tmp_R0" (BType_Imm Bit32); BVar "sy_tmp_PSR_Z" (BType_Imm Bit1);
- BVar "sy_tmp_PSR_V" (BType_Imm Bit1); BVar "sy_tmp_PSR_N" (BType_Imm Bit1);
- BVar "sy_tmp_PSR_C" (BType_Imm Bit1);
- BVar "sy_tmp_MEM" (BType_Mem Bit32 Bit8);
- BVar "sy_tmp_COND" (BType_Imm Bit1); BVar "sy_tmp_PC" (BType_Imm Bit32);
- BVar "sy_countw" (BType_Imm Bit64); BVar "sy_ModeHandler" (BType_Imm Bit1);
- BVar "sy_SP_process" (BType_Imm Bit32); BVar "sy_SP_main" (BType_Imm Bit32);
- BVar "sy_LR" (BType_Imm Bit32); BVar "sy_R12" (BType_Imm Bit32);
- BVar "sy_R11" (BType_Imm Bit32); BVar "sy_R10" (BType_Imm Bit32);
- BVar "sy_R9" (BType_Imm Bit32); BVar "sy_R8" (BType_Imm Bit32);
- BVar "sy_R7" (BType_Imm Bit32); BVar "sy_R6" (BType_Imm Bit32);
- BVar "sy_R5" (BType_Imm Bit32); BVar "sy_R4" (BType_Imm Bit32);
- BVar "sy_R3" (BType_Imm Bit32); BVar "sy_R2" (BType_Imm Bit32);
- BVar "sy_R1" (BType_Imm Bit32); BVar "sy_R0" (BType_Imm Bit32);
- BVar "sy_PSR_Z" (BType_Imm Bit1); BVar "sy_PSR_V" (BType_Imm Bit1);
- BVar "sy_PSR_N" (BType_Imm Bit1); BVar "sy_PSR_C" (BType_Imm Bit1);
- BVar "sy_MEM" (BType_Mem Bit32 Bit8)} ∩
-({BVar "sy_countw" (BType_Imm Bit64); BVar "sy_SP_process" (BType_Imm Bit32);
-  BVar "sy_SP_process" (BType_Imm Bit32);
-  BVar "sy_SP_process" (BType_Imm Bit32);
-  BVar "sy_SP_process" (BType_Imm Bit32);
-  BVar "sy_SP_process" (BType_Imm Bit32);
-  BVar "sy_SP_process" (BType_Imm Bit32);
-  BVar "sy_tmp_countw" (BType_Imm Bit64);
-  BVar "sy_tmp_ModeHandler" (BType_Imm Bit1);
-  BVar "sy_tmp_SP_main" (BType_Imm Bit32);
-  BVar "sy_tmp_LR" (BType_Imm Bit32); BVar "sy_tmp_R12" (BType_Imm Bit32);
-  BVar "sy_tmp_R11" (BType_Imm Bit32); BVar "sy_tmp_R10" (BType_Imm Bit32);
-  BVar "sy_tmp_R9" (BType_Imm Bit32); BVar "sy_tmp_R8" (BType_Imm Bit32);
-  BVar "sy_tmp_R7" (BType_Imm Bit32); BVar "sy_tmp_R6" (BType_Imm Bit32);
-  BVar "sy_tmp_R5" (BType_Imm Bit32); BVar "sy_tmp_R4" (BType_Imm Bit32);
-  BVar "sy_tmp_R3" (BType_Imm Bit32); BVar "sy_tmp_R2" (BType_Imm Bit32);
-  BVar "sy_tmp_R1" (BType_Imm Bit32); BVar "sy_tmp_R0" (BType_Imm Bit32);
-  BVar "sy_tmp_PSR_Z" (BType_Imm Bit1); BVar "sy_tmp_PSR_V" (BType_Imm Bit1);
-  BVar "sy_tmp_PSR_N" (BType_Imm Bit1); BVar "sy_tmp_PSR_C" (BType_Imm Bit1);
-  BVar "sy_tmp_MEM" (BType_Mem Bit32 Bit8);
-  BVar "sy_tmp_COND" (BType_Imm Bit1); BVar "sy_tmp_PC" (BType_Imm Bit32);
-  BVar "sy_ModeHandler" (BType_Imm Bit1);
-  BVar "sy_SP_process" (BType_Imm Bit32);
-  BVar "sy_SP_main" (BType_Imm Bit32); BVar "sy_LR" (BType_Imm Bit32);
-  BVar "sy_R12" (BType_Imm Bit32); BVar "sy_R11" (BType_Imm Bit32);
-  BVar "sy_R10" (BType_Imm Bit32); BVar "sy_R9" (BType_Imm Bit32);
-  BVar "sy_R8" (BType_Imm Bit32); BVar "sy_R7" (BType_Imm Bit32);
-  BVar "sy_R6" (BType_Imm Bit32); BVar "sy_R5" (BType_Imm Bit32);
-  BVar "sy_R4" (BType_Imm Bit32); BVar "sy_R3" (BType_Imm Bit32);
-  BVar "sy_R2" (BType_Imm Bit32); BVar "sy_R1" (BType_Imm Bit32);
-  BVar "sy_R0" (BType_Imm Bit32); BVar "sy_PSR_Z" (BType_Imm Bit1);
-  BVar "sy_PSR_V" (BType_Imm Bit1); BVar "sy_PSR_N" (BType_Imm Bit1);
-  BVar "sy_PSR_C" (BType_Imm Bit1); BVar "sy_MEM" (BType_Mem Bit32 Bit8);
-  BVar "sy_SP_process" (BType_Imm Bit32); BVar "sy_countw" (BType_Imm Bit64)} DIFF
- {BVar "sy_countw" (BType_Imm Bit64); BVar "sy_SP_process" (BType_Imm Bit32);
-  BVar "sy_SP_process" (BType_Imm Bit32);
-  BVar "sy_SP_process" (BType_Imm Bit32);
-  BVar "sy_SP_process" (BType_Imm Bit32);
-  BVar "sy_SP_process" (BType_Imm Bit32);
-  BVar "sy_SP_process" (BType_Imm Bit32);
-  BVar "sy_tmp_countw" (BType_Imm Bit64);
-  BVar "sy_tmp_ModeHandler" (BType_Imm Bit1);
-  BVar "sy_tmp_SP_main" (BType_Imm Bit32);
-  BVar "sy_tmp_LR" (BType_Imm Bit32); BVar "sy_tmp_R12" (BType_Imm Bit32);
-  BVar "sy_tmp_R11" (BType_Imm Bit32); BVar "sy_tmp_R10" (BType_Imm Bit32);
-  BVar "sy_tmp_R9" (BType_Imm Bit32); BVar "sy_tmp_R8" (BType_Imm Bit32);
-  BVar "sy_tmp_R7" (BType_Imm Bit32); BVar "sy_tmp_R6" (BType_Imm Bit32);
-  BVar "sy_tmp_R5" (BType_Imm Bit32); BVar "sy_tmp_R4" (BType_Imm Bit32);
-  BVar "sy_tmp_R3" (BType_Imm Bit32); BVar "sy_tmp_R2" (BType_Imm Bit32);
-  BVar "sy_tmp_R1" (BType_Imm Bit32); BVar "sy_tmp_R0" (BType_Imm Bit32);
-  BVar "sy_tmp_PSR_Z" (BType_Imm Bit1); BVar "sy_tmp_PSR_V" (BType_Imm Bit1);
-  BVar "sy_tmp_PSR_N" (BType_Imm Bit1); BVar "sy_tmp_PSR_C" (BType_Imm Bit1);
-  BVar "sy_tmp_MEM" (BType_Mem Bit32 Bit8);
-  BVar "sy_tmp_COND" (BType_Imm Bit1); BVar "sy_tmp_PC" (BType_Imm Bit32);
-  BVar "sy_countw" (BType_Imm Bit64); BVar "sy_ModeHandler" (BType_Imm Bit1);
-  BVar "sy_SP_process" (BType_Imm Bit32);
-  BVar "sy_SP_main" (BType_Imm Bit32); BVar "sy_LR" (BType_Imm Bit32);
-  BVar "sy_R12" (BType_Imm Bit32); BVar "sy_R11" (BType_Imm Bit32);
-  BVar "sy_R10" (BType_Imm Bit32); BVar "sy_R9" (BType_Imm Bit32);
-  BVar "sy_R8" (BType_Imm Bit32); BVar "sy_R7" (BType_Imm Bit32);
-  BVar "sy_R6" (BType_Imm Bit32); BVar "sy_R5" (BType_Imm Bit32);
-  BVar "sy_R4" (BType_Imm Bit32); BVar "sy_R3" (BType_Imm Bit32);
-  BVar "sy_R2" (BType_Imm Bit32); BVar "sy_R1" (BType_Imm Bit32);
-  BVar "sy_R0" (BType_Imm Bit32); BVar "sy_PSR_Z" (BType_Imm Bit1);
-  BVar "sy_PSR_V" (BType_Imm Bit1); BVar "sy_PSR_N" (BType_Imm Bit1);
-  BVar "sy_PSR_C" (BType_Imm Bit1); BVar "sy_MEM" (BType_Mem Bit32 Bit8);
-  BVar "sy_SP_process" (BType_Imm Bit32)}) ⊆ ∅
-``,
-);
-*)
-
 
       CONV_TAC (RATOR_CONV (RAND_CONV (bir_vars_ofLib.freevarset_CONV))) >>
       (fn (al,g) => (print "finished to proof free symbols operation\n"; ([(al,g)], fn ([t]) => t))) >>
@@ -261,28 +143,18 @@ val freesymbols_B_thm_o = SOME (prove(T, cheat));
 *)
 fun birs_rule_SEQ_fun (birs_rule_SEQ_thm, bprog_tm) step_A_thm step_B_thm freesymbols_B_thm_o =
   let
-    val symb_struct_get_bprog_fun = snd o dest_comb o hd o snd o strip_comb;
-    val bprog_A_tm = (symb_struct_get_bprog_fun o concl) step_A_thm;
-    val bprog_B_tm = (symb_struct_get_bprog_fun o concl) step_B_thm;
+    val (bprog_A_tm,_) = (dest_birs_symb_exec o concl) step_A_thm;
+    val (bprog_B_tm,_) = (dest_birs_symb_exec o concl) step_B_thm;
     val _ = if identical bprog_tm bprog_A_tm andalso identical bprog_tm bprog_B_tm then () else
             raise Fail "birs_rule_SEQ_fun:: the programs have to match";
-
-    (*
-    val (sys_A_tm, _, _)       = (symb_sound_struct_get_sysLPi_fun o concl) step_A_thm;
-    val (sys_B_tm, _, Pi_B_tm) = (symb_sound_struct_get_sysLPi_fun o concl) step_B_thm;
-    *)
 
     val prep_thm =
       HO_MATCH_MP (HO_MATCH_MP birs_rule_SEQ_thm step_A_thm) step_B_thm;
 
-    (* has to solve this implication ((birs_symb_symbols bsys_A) INTER (birs_freesymbs bsys_B bPi_B) = EMPTY) *)
-    val freesymbols_tm = (hd o fst o strip_imp o concl) prep_thm;
+    (* has to solve this ((birs_symb_symbols bsys_A) INTER (birs_freesymbs bsys_B bPi_B) = EMPTY) *)
+    val freesymbols_tm = (fst o dest_imp o concl) prep_thm;
     val freesymbols_thm = birs_rule_SEQ_free_symbols_fun freesymbols_tm freesymbols_B_thm_o;
     val _ = print "finished to proof free symbols altogether\n";
-    (*
-    val bprog_composed_thm = save_thm(
-       "bprog_composed_thm",
-    *)
 
     val bprog_composed_thm =
            (MATCH_MP
@@ -290,53 +162,19 @@ fun birs_rule_SEQ_fun (birs_rule_SEQ_thm, bprog_tm) step_A_thm step_B_thm freesy
               freesymbols_thm);
     val _ = print "composed\n";
 
-    (* TODO: tidy up set operations to not accumulate (in both, post state set and label set) - does this simplification work well enough? *)
-    (* val bprog_composed_thm_ = SIMP_RULE (std_ss++pred_setLib.PRED_SET_ss) [] bprog_composed_thm; *)
-    (* val bprog_composed_thm_ = SIMP_RULE (std_ss++pred_setLib.PRED_SET_ss++HolBACoreSimps.holBACore_ss) [pred_setTheory.INSERT_UNION] bprog_composed_thm; *)
-
-(*
-val tm = (snd o dest_comb o snd o dest_comb o snd o dest_comb o concl) bprog_composed_thm;
-*)
-
-(*
-    val conv = aux_setLib.birs_state_DIFF_UNION_CONV;
-*)
+    (* tidy up set operations to not accumulate (in both, post state set and label set) *)
     fun Pi_CONV conv tm =
       RAND_CONV (RAND_CONV (conv handle e => (print "\n\nPi_CONV failed\n\n"; raise e))) tm;
-
     fun L_CONV conv tm =
       RAND_CONV (LAND_CONV (conv handle e => (print "\n\nL_CONV failed\n\n"; raise e))) tm;
 
     val bprog_Pi_fixed_thm = CONV_RULE (RAND_CONV (Pi_CONV aux_setLib.birs_state_DIFF_UNION_CONV)) bprog_composed_thm;
 
     val bprog_L_fixed_thm  = CONV_RULE (RAND_CONV (L_CONV (
-      EVAL (* TODO: this has to be fixed as list of address spaces that can be merged and so on... (can we make this only involve the block label part, not the block index?) *)
-      (*SIMP_CONV
-        (std_ss++HolBACoreSimps.holBACore_ss++birs_state_ss++pred_setLib.PRED_SET_ss++wordsLib.WORD_ss)
-        [bir_symbTheory.birs_symb_to_symbst_EQ_thm, pred_setTheory.INSERT_UNION]*)
+      EVAL
+      (* TODO: this has to be fixed as list of address spaces that can be merged and so on...
+         (can we make this only involve the block label part, not the block index?) *)
         ))) bprog_Pi_fixed_thm;
-
-(*
-    val bprog_composed_thm_1 =
-      (SIMP_RULE
-        (std_ss++HolBACoreSimps.holBACore_ss++birs_state_ss++pred_setLib.PRED_SET_ss)
-        [bir_symbTheory.birs_symb_to_symbst_EQ_thm, pred_setTheory.INSERT_UNION]
-        bprog_composed_thm);
-    val _ = print "UNION\n";
-
-    (* reconstruct IMAGE in the post state set *)
-    val IMAGE_EMPTY_thm =
-      Q.SPEC `birs_symb_to_symbst` (
-        INST_TYPE [beta |-> Type`:(bir_programcounter_t, string, bir_exp_t, bir_status_t) symb_symbst_t`, alpha |-> Type`:birs_state_t`] 
-        pred_setTheory.IMAGE_EMPTY
-      );
-    val _ = print "FIX\n";
-    val bprog_composed_thm_2 =
-      CONV_RULE
-        (PAT_CONV ``\A. symb_hl_step_in_L_sound B (C, D, A)`` (REWRITE_CONV [GSYM IMAGE_EMPTY_thm, GSYM pred_setTheory.IMAGE_INSERT]))
-        bprog_composed_thm_1
-    val _ = print "IMAGE_INSERT\n";
-*)
 
     val _ = if symb_sound_struct_is_normform (concl bprog_L_fixed_thm) then () else
             (print_term (concl bprog_L_fixed_thm);
